---
layout: post
title: Implicit Derivatives
date: 2015-10-07
tags:
  - test
  - math
---

take the equation
$$
4 = x^2 + y^2
$$

Even though we can solve this for $$ y $$, we'll assume that we can't so we can showcase implicit derivatives.

An **implicitly defined function** is a function that takes the form $$ x^2 + y^2 = 1 $$, this example is the unit circle function.

To take derivatives of these functions, we need to treat $$ y $$ as a function of $$ x $$.

With $$ y $$ being a function of $$ x $$, we can use the **chain rule** to take the derivative of it, then treat $$ \frac{dy}{dx} $$ or $$ f' $$ as an algebraic variable.

The best way to learn this is to do problems, so let's do one.

1. *Take the derivative of the function and find the equation of the tangent line at $$ (1,-4) $$*

$$

\begin{align*} 

4 &= x^2 + y^2 \\
\frac{d}{dx}4 &= \frac{d}{dx}x^2 + \frac{d}{dx}y^2

\end{align*}
$$

1. constant rule, so $$ \frac{d}{dx}4 = 0 $$
2. power rule, so $$ \frac{d}{dx}x^2  = {2x^1} $$
3. now comes the hard part. The variables disagree, we have to use the chain rule

$$
\frac{d}{d \color{red}{x}}\color{red}{y}^2
$$

when using the chain rule, we get

$$
2(y)\cdot \frac{dy}{dx}
$$

Now, let's put it all together and do some algebra

$$
0 = 2x + 2y\frac{dy}{dx}
$$

Subtract $$ 2x $$ from both sides

$$
2y\frac{dy}{dx} = -2x
$$

Divide by $$ 2y $$

$$
\frac{dy}{dx} = \frac{-2x}{2y}
$$

Simplify, and done

$$
\frac{dy}{dx} = \frac{-x}{y}
$$

Now to find the tangent line at $$ (1,-4) $$

$$
\begin{align*} 
y+4&=\frac{1}{4}(x+1) \\
y &= \frac{1}{4}x - \frac{3}{4}
\end{align*}
$$
